@prefix dct: <http://purl.org/dc/terms/> .
@prefix foaf: <http://xmlns.com/foaf/0.1/> .
@prefix rdf: <http://www.w3.org/1999/02/22-rdf-syntax-ns#> .
@prefix skos: <http://www.w3.org/2004/02/skos/core#> .
@prefix vocab: <http://purl.org/m4m21/subjects/> .
@prefix xsd: <http://www.w3.org/2001/XMLSchema#> .
@prefix rdfs: <http://www.w3.org/2000/01/rdf-schema#> .
@prefix owl: <http://www.w3.org/2002/07/owl#> .
@prefix schema: <http://schema.org/>.
@prefix iop:   <https://w3id.org/iadopt/ont/> .
@prefix puv: <https://w3id.org/env/puv#> .
@prefix sosa: <http://www.w3.org/ns/sosa/> .

iop:constrains  a     owl:ObjectProperty ;
        rdfs:comment  "A Constraint constrains an Entity having a role in the Variable description." ;
        rdfs:domain   iop:Constraint ;
        rdfs:label    "constrains" ;
        rdfs:range    iop:Entity .

iop:hasConstraint  a  owl:ObjectProperty ;
        rdfs:comment  "A Variable has a Constraint, that confines an Entity involved in the observation." ;
        rdfs:domain   iop:Variable ;
        rdfs:label    "hasConstraint" ;
        rdfs:range    iop:Constraint .

iop:hasContextObject  a  owl:ObjectProperty ;
        rdfs:comment  "A Variable has an Entity that provides additional background information regarding the ObjectOfInterest." ;
        rdfs:domain   iop:Variable ;
        rdfs:label    "hasContextObject" ;
        rdfs:range    iop:Entity .

iop:hasMatrix  a            owl:ObjectProperty ;
        rdfs:comment        "A Variable might have an Entity in which the ObjectOfInterest is contained." ;
        rdfs:domain         iop:Variable ;
        rdfs:label          "hasMatrix" ;
        rdfs:range          iop:Entity ;
        rdfs:subPropertyOf  iop:hasContextObject .

iop:hasObjectOfInterest
        a             owl:ObjectProperty ;
        rdfs:comment  "A Variable has an Entity whose Property is observed." ;
        rdfs:domain   iop:Variable ;
        rdfs:label    "hasObjectOfInterest" ;
        rdfs:range    iop:Entity .

iop:hasProperty  a    owl:ObjectProperty ;
        rdfs:comment  "A Variable has a Property that characterizes an Entity." ;
        rdfs:domain   iop:Variable ;
        rdfs:label    "hasProperty" ;
        rdfs:range    iop:Property .

puv:uom
  a owl:ObjectProperty ;
  rdfs:comment "scale or unit of measurement" ;
  rdfs:label "unit-of-measurement " ;
  rdfs:range puv:UnitOfMeasurement .

puv:statistic
  a owl:ObjectProperty ;
  rdfs:comment "statistical treatment" ;
  rdfs:domain puv:Parameter ;
  rdfs:label "statistic " ;
  rdfs:range puv:ParameterStatistic .

puv:method
  a owl:ObjectProperty ;
  rdfs:comment "method used to measure the value" ;
  rdfs:label "method" ;
  rdfs:range puv:Method .
        
sosa:madeBySensor 
  a owl:ObjectProperty ;
  rdfs:label "made by sensor"@en ;
  skos:definition "Relation between an Observation and the Sensor which made the Observation."@en ;
  rdfs:comment "Relation between an Observation and the Sensor which made the Observation."@en ;
  schema:domainIncludes sosa:Observation ;
  schema:rangeIncludes sosa:Sensor ;
  owl:inverseOf sosa:madeObservation ;
  rdfs:isDefinedBy sosa: .

<http://purl.org/m4m21/subjects> a skos:ConceptScheme;
  dct:created "2022-06-01T00:00:00+00:00"^^xsd:datetime;
  dct:description "Vocabulary description"@en;
  dct:hasVersion "0.1.0";
  dct:modified "2022-06-11T18:39:12+00:00"^^xsd:datetime;
  dct:rights <https://spdx.org/licenses/CC0-1.0>;
  dct:title "Vocabulary title"@en;
  skos:hasTopConcept vocab:1000, vocab:1002;
  foaf:homepage "URL to the community developing vocab"@en .

vocab:1000 a skos:Concept;
  skos:altLabel "Test Subject Alternative Label"@en;
  skos:definition "Test Subject Definition"@en;
  skos:inScheme <http://purl.org/m4m21/subjects>;
  skos:narrower vocab:1001;
  skos:prefLabel "Test Top Subject"@en;
  skos:topConceptOf <http://purl.org/m4m21/subjects> .

vocab:1001 a skos:Concept;
  skos:broader vocab:1000;
  skos:inScheme <http://purl.org/m4m21/subjects>;
  skos:prefLabel "Test Narrow Subject"@en .

vocab:1002 a skos:Concept;
  skos:inScheme <http://purl.org/m4m21/subjects>;
  skos:narrower vocab:1003;
  skos:prefLabel "Test Top Subject 2"@en;
  skos:topConceptOf <http://purl.org/m4m21/subjects> .

vocab:1003 a skos:Concept;
  skos:broader vocab:1002;
  skos:inScheme <http://purl.org/m4m21/subjects>;
  skos:prefLabel "Test Narrow Subject 2"@en .
